backends/lean/Aeneas/Tactic/Step/Tests/SpecPartial.lean
@@ -56,8 +56,7 @@ info: Aeneas.Step.SpecPartialTests.myDiv_spec_partial.mvcgen_spec (x y : U32) (Q
   (h_ok : ∀ (r : U32), ↑r = ↑x / ↑y → willYield r Q) (h_fail_1 : ↑y = 0 → willFail Error.assertionFailure Q)
   (h_fail_2 : ↑y = 0 → willFail Error.integerOverflow Q) (h_fail_3 : ↑y = 0 → willFail Error.divisionByZero Q)
   (h_fail_4 : ↑y = 0 → willFail Error.arrayOutOfBounds Q) (h_fail_5 : ↑y = 0 → willFail Error.maximumSizeExceeded Q)
-  (h_fail_6 : ↑y = 0 → willFail Error.panic Q) (h_fail_7 : ↑y = 0 → willFail Error.undef Q) :
-  ⦃⌜True⌝⦄ myDiv x y ⦃Q⦄
+  (h_fail_6 : ↑y = 0 → willFail Error.panic Q) (h_fail_7 : ↑y = 0 → willFail Error.undef Q) : ⦃⌜True⌝⦄ myDiv x y ⦃Q⦄
 -/
 #guard_msgs in
 #check myDiv_spec_partial.mvcgen_spec
